---
title     : "TypedBadfix: Typed Lambda term representation (bad fix)"
permalink : /TypedBadfix
---


## Imports

\begin{code}
module TypedBadfix where
\end{code}

\begin{code}
import Relation.Binary.PropositionalEquality as Eq
open Eq using (_≡_; refl; sym; trans; cong; cong₂; _≢_)
open import Data.Empty using (⊥; ⊥-elim)
open import Data.List using (List; []; _∷_; [_]; _++_; map; foldr; filter)
open import Data.List.Any using (Any; here; there)
open import Data.Nat using (ℕ; zero; suc; _+_; _∸_; _≤_; _⊔_; _≟_)
open import Data.Nat.Properties using (≤-refl; ≤-trans; m≤m⊔n; n≤m⊔n; 1+n≰n)
open import Data.Product using (_×_; proj₁; proj₂; ∃; ∃-syntax)
              renaming (_,_ to ⟨_,_⟩)
open import Data.Sum using (_⊎_; inj₁; inj₂)
open import Data.Unit using (⊤; tt)
open import Function using (_∘_)
open import Function.Equality using (≡-setoid)
open import Function.Equivalence using (_⇔_; equivalence)
open import Relation.Nullary using (¬_; Dec; yes; no)
open import Relation.Nullary.Negation using (contraposition; ¬?)
open import Relation.Nullary.Product using (_×-dec_)
import Collections
\end{code}


## Syntax

\begin{code}
infixr 5 _⟹_
infixl 5 _,_⦂_
infix  4 _∋_⦂_
infix  4 _⊢_⦂_
infix  5 `λ_⇒_
infix  5 `λ_
infixl 6 _·_
infix  7 `_

Id : Set
Id = ℕ

data Type : Set where
  `ℕ  : Type
  _⟹_ : Type → Type → Type

data Env : Set where
  ε     : Env
  _,_⦂_ : Env → Id → Type → Env

data Term : Set where
  `_    : Id → Term
  `λ_⇒_ : Id → Term → Term
  _·_   : Term → Term → Term

data _∋_⦂_ : Env → Id → Type → Set where

  Z : ∀ {Γ A x}
      -----------------
    → Γ , x ⦂ A ∋ x ⦂ A

  S : ∀ {Γ A B x w}
    → w ≢ x
    → Γ ∋ w ⦂ B
      -----------------
    → Γ , x ⦂ A ∋ w ⦂ B

data _⊢_⦂_ : Env → Term → Type → Set where

  `_ : ∀ {Γ A x}
    → Γ ∋ x ⦂ A
      ---------------------
    → Γ ⊢ ` x ⦂ A

  `λ_ : ∀ {Γ x A N B}
    → Γ , x ⦂ A ⊢ N ⦂ B
      ------------------------
    → Γ ⊢ (`λ x ⇒ N) ⦂ A ⟹ B

  _·_ : ∀ {Γ L M A B}
    → Γ ⊢ L ⦂ A ⟹ B
    → Γ ⊢ M ⦂ A
      --------------
    → Γ ⊢ L · M ⦂ B
\end{code}

## Test examples

\begin{code}
m n s z : Id
m = 0
n = 1
s = 2
z = 3

s≢z : s ≢ z
s≢z ()

n≢z : n ≢ z
n≢z ()

n≢s : n ≢ s
n≢s ()

m≢z : m ≢ z
m≢z ()

m≢s : m ≢ s
m≢s ()

m≢n : m ≢ n
m≢n ()

Ch : Type
Ch = (`ℕ ⟹ `ℕ) ⟹ `ℕ ⟹ `ℕ

two : Term
two = `λ s ⇒ `λ z ⇒ (` s · (` s · ` z))

⊢two : ε ⊢ two ⦂ Ch
⊢two = `λ `λ ` ⊢s · (` ⊢s · ` ⊢z)
  where
  ⊢s = S s≢z Z
  ⊢z = Z

four : Term
four = `λ s ⇒ `λ z ⇒ ` s · (` s · (` s · (` s · ` z)))

⊢four : ε ⊢ four ⦂ Ch
⊢four = `λ `λ ` ⊢s · (` ⊢s · (` ⊢s · (` ⊢s · ` ⊢z)))
  where
  ⊢s = S s≢z Z
  ⊢z = Z

plus : Term
plus = `λ m ⇒ `λ n ⇒ `λ s ⇒ `λ z ⇒ ` m · ` s · (` n · ` s · ` z)

⊢plus : ε ⊢ plus ⦂ Ch ⟹ Ch ⟹ Ch
⊢plus = `λ `λ `λ `λ  ` ⊢m ·  ` ⊢s · (` ⊢n · ` ⊢s · ` ⊢z)
  where
  ⊢z = Z
  ⊢s = S s≢z Z
  ⊢n = S n≢z (S n≢s Z)
  ⊢m = S m≢z (S m≢s (S m≢n Z))

four′ : Term
four′ = plus · two · two

⊢four′ : ε ⊢ four′ ⦂ Ch
⊢four′ = ⊢plus · ⊢two · ⊢two
\end{code}


# Denotational semantics

\begin{code}
⟦_⟧ᵀ : Type → Set
⟦ `ℕ ⟧ᵀ     =  ℕ
⟦ A ⟹ B ⟧ᵀ  =  ⟦ A ⟧ᵀ → ⟦ B ⟧ᵀ

⟦_⟧ᴱ : Env → Set
⟦ ε ⟧ᴱ          =  ⊤
⟦ Γ , x ⦂ A ⟧ᴱ  =  ⟦ Γ ⟧ᴱ × ⟦ A ⟧ᵀ

⟦_⟧ⱽ : ∀ {Γ x A} → Γ ∋ x ⦂ A → ⟦ Γ ⟧ᴱ → ⟦ A ⟧ᵀ
⟦ Z ⟧ⱽ     ⟨ ρ , v ⟩ = v
⟦ S _ x ⟧ⱽ ⟨ ρ , v ⟩ = ⟦ x ⟧ⱽ ρ

⟦_⟧ : ∀ {Γ M A} → Γ ⊢ M ⦂ A → ⟦ Γ ⟧ᴱ → ⟦ A ⟧ᵀ
⟦ ` x ⟧     ρ  =  ⟦ x ⟧ⱽ ρ
⟦ `λ ⊢N ⟧   ρ  =  λ{ v → ⟦ ⊢N ⟧ ⟨ ρ , v ⟩ }
⟦ ⊢L · ⊢M ⟧ ρ  =  (⟦ ⊢L ⟧ ρ) (⟦ ⊢M ⟧ ρ)

_ : ⟦ ⊢four′ ⟧ tt ≡ ⟦ ⊢four ⟧ tt
_ = refl

_ : ⟦ ⊢four ⟧ tt suc zero ≡ 4
_ = refl
\end{code}


## Erasure

\begin{code}
lookup : ∀ {Γ x A} → Γ ∋ x ⦂ A → Id
lookup {Γ , x ⦂ A} Z        =  x
lookup {Γ , x ⦂ A} (S _ k)  =  lookup {Γ} k

erase : ∀ {Γ M A} → Γ ⊢ M ⦂ A → Term
erase (` k)              =  ` lookup k
erase (`λ_ {x = x} ⊢N)   =  `λ x ⇒ erase ⊢N
erase (⊢L · ⊢M)          =  erase ⊢L · erase ⊢M
\end{code}

### Properties of erasure

\begin{code}
lookup-lemma : ∀ {Γ x A} → (⊢x : Γ ∋ x ⦂ A) → lookup ⊢x ≡ x
lookup-lemma Z        =  refl
lookup-lemma (S _ k)  =  lookup-lemma k

erase-lemma : ∀ {Γ M A} → (⊢M : Γ ⊢ M ⦂ A) → erase ⊢M ≡ M
erase-lemma (` ⊢x)            =  cong `_ (lookup-lemma ⊢x)
erase-lemma (`λ_ {x = x} ⊢N)  =  cong (`λ x ⇒_) (erase-lemma ⊢N)
erase-lemma (⊢L · ⊢M)         =  cong₂ _·_ (erase-lemma ⊢L) (erase-lemma ⊢M)
\end{code}


## Substitution

### Lists as sets

\begin{code}
open Collections (Id) (_≟_)
\end{code}

### Free variables

\begin{code}
free : Term → List Id
free (` x)       =  [ x ]
free (`λ x ⇒ N)  =  free N \\ x
free (L · M)     =  free L ++ free M
\end{code}

### Fresh identifier

\begin{code}
fresh : List Id → Id
fresh = foldr _⊔_ 0 ∘ map suc

⊔-lemma : ∀ {w xs} → w ∈ xs → suc w ≤ fresh xs
⊔-lemma {_} {_ ∷ xs} here        =  m≤m⊔n _ (fresh xs)
⊔-lemma {_} {_ ∷ xs} (there x∈)  =  ≤-trans (⊔-lemma x∈) (n≤m⊔n _ (fresh xs))

fresh-lemma : ∀ {x xs} → x ∈ xs → x ≢ fresh xs
fresh-lemma x∈ refl =  1+n≰n (⊔-lemma x∈)
\end{code}

### Identifier maps

\begin{code}
∅ : Id → Term
∅ x = ` x

infixl 5 _,_↦_

_,_↦_ : (Id → Term) → Id → Term → (Id → Term)
(ρ , x ↦ M) w with w ≟ x
...               | yes _   =  M
...               | no  _   =  ρ w
\end{code}

### Substitution

\begin{code}
subst : List Id → (Id → Term) → Term → Term
subst ys ρ (` x)          =  ρ x
subst ys ρ (`λ x ⇒ N)     =  `λ y ⇒ subst (y ∷ ys) (ρ , x ↦ ` y) N
  where
  y = fresh ys
subst ys ρ (L · M)        =  subst ys ρ L · subst ys ρ M

_[_:=_] : Term → Id → Term → Term
N [ x := M ]  =  subst (free M ++ (free N \\ x)) (∅ , x ↦ M) N
\end{code}


## Values

\begin{code}
data Value : Term → Set where

  Fun : ∀ {x N}
      ---------------
    → Value (`λ x ⇒ N)
\end{code}

## Reduction

\begin{code}
infix 4 _⟶_

data _⟶_ : Term → Term → Set where

  β-⟹ : ∀ {x N V}
    → Value V
      ------------------------------
    → (`λ x ⇒ N) · V ⟶ N [ x := V ]

  ξ-⟹₁ : ∀ {L L′ M}
    → L ⟶ L′
      ----------------
    → L · M ⟶ L′ · M

  ξ-⟹₂ : ∀ {V M M′} →
    Value V →
    M ⟶ M′ →
    ----------------
    V · M ⟶ V · M′
\end{code}

## Reflexive and transitive closure

\begin{code}
infix  2 _⟶*_
infix 1 begin_
infixr 2 _⟶⟨_⟩_
infix 3 _∎

data _⟶*_ : Term → Term → Set where

  _∎ : ∀ {M}
      -------------
    → M ⟶* M

  _⟶⟨_⟩_ : ∀ (L : Term) {M N}
    → L ⟶ M
    → M ⟶* N
      ---------
    → L ⟶* N

begin_ : ∀ {M N} → (M ⟶* N) → (M ⟶* N)
begin M⟶*N = M⟶*N
\end{code}

## Progress

\begin{code}
data Progress (M : Term) : Set where
  step : ∀ {N}
    → M ⟶ N
      ----------
    → Progress M
  done :
      Value M
      ----------
    → Progress M

progress : ∀ {M A} → ε ⊢ M ⦂ A → Progress M
progress (` ())
progress (`λ_ ⊢N)                                         =  done Fun
progress (⊢L · ⊢M) with progress ⊢L
...                   | step L⟶L′                       =  step (ξ-⟹₁ L⟶L′)
...                   | done Fun      with progress ⊢M
...                                      | step M⟶M′    =  step (ξ-⟹₂ Fun M⟶M′)
...                                      | done valM      =  step (β-⟹ valM)
\end{code}


## Preservation

### Domain of an environment

\begin{code}
dom : Env → List Id
dom ε            =  []
dom (Γ , x ⦂ A)  =  x ∷ dom Γ

dom-lemma : ∀ {Γ y B} → Γ ∋ y ⦂ B → y ∈ dom Γ
dom-lemma Z           =  here
dom-lemma (S x≢y ⊢y)  =  there (dom-lemma ⊢y)

free-lemma : ∀ {Γ M A} → Γ ⊢ M ⦂ A → free M ⊆ dom Γ
free-lemma (` ⊢x) w∈ with w∈
...                     | here          =  dom-lemma ⊢x
...                     | there ()
free-lemma {Γ} (`λ_ {x = x} {N = N} ⊢N)  =  ∷-to-\\ (free-lemma ⊢N)
free-lemma (⊢L · ⊢M) w∈ with ++-to-⊎ w∈
...                        | inj₁ ∈L    = free-lemma ⊢L ∈L
...                        | inj₂ ∈M    = free-lemma ⊢M ∈M
\end{code}

### Weakening

\begin{code}
⊢weaken : ∀ {Γ Δ}
  → (∀ {x A} → Γ ∋ x ⦂ A  →  Δ ∋ x ⦂ A)
    --------------------------------------------------
  → (∀ {M A} → Γ ⊢ M ⦂ A  →  Δ ⊢ M ⦂ A)
⊢weaken ⊢σ (` ⊢x)     =  ` ⊢σ ⊢x
⊢weaken {Γ} {Δ} ⊢σ (`λ_ {x = x} {A = A} {N = N} ⊢N)
                          =  `λ (⊢weaken {Γ′} {Δ′} ⊢σ′ ⊢N)
  where
  Γ′   =  Γ , x ⦂ A
  Δ′   =  Δ , x ⦂ A

  ⊢σ′ : ∀ {w B} → Γ′ ∋ w ⦂ B → Δ′ ∋ w ⦂ B
  ⊢σ′ Z          =  Z
  ⊢σ′ (S w≢ ⊢w)  =  S w≢ (⊢σ ⊢w)

⊢weaken ⊢σ (⊢L · ⊢M)  =  ⊢weaken ⊢σ ⊢L · ⊢weaken ⊢σ ⊢M
\end{code}

### Strengthening is old renaming

### Renaming

\begin{code}
⊢rename : ∀ {Γ Δ xs}
  → (∀ {x A} → x ∈ xs      →  Γ ∋ x ⦂ A  →  Δ ∋ x ⦂ A)
    --------------------------------------------------
  → (∀ {M A} → free M ⊆ xs →  Γ ⊢ M ⦂ A  →  Δ ⊢ M ⦂ A)
⊢rename ⊢σ ⊆xs (` ⊢x)     =  ` ⊢σ ∈xs ⊢x
  where
  ∈xs = ⊆xs here
⊢rename {Γ} {Δ} {xs} ⊢σ ⊆xs (`λ_ {x = x} {A = A} {N = N} ⊢N)
                          =  `λ (⊢rename {Γ′} {Δ′} {xs′} ⊢σ′ ⊆xs′ ⊢N)
  where
  Γ′   =  Γ , x ⦂ A
  Δ′   =  Δ , x ⦂ A
  xs′  =  x ∷ xs

  ⊢σ′ : ∀ {w B} → w ∈ xs′ → Γ′ ∋ w ⦂ B → Δ′ ∋ w ⦂ B
  ⊢σ′ w∈′ Z          =  Z
  ⊢σ′ w∈′ (S w≢ ⊢w)  =  S w≢ (⊢σ ∈w ⊢w)
    where
    ∈w  =  there⁻¹ w∈′ w≢

  ⊆xs′ : free N ⊆ xs′
  ⊆xs′ = \\-to-∷ ⊆xs
⊢rename ⊢σ ⊆xs (⊢L · ⊢M)  =  ⊢rename ⊢σ L⊆ ⊢L · ⊢rename ⊢σ M⊆ ⊢M
  where
  L⊆ = trans-⊆ ⊆-++₁ ⊆xs
  M⊆ = trans-⊆ ⊆-++₂ ⊆xs
\end{code}


### Substitution preserves types, general case

\begin{code}
map-≡ : ∀ {ρ M w x} → w ≡ x → (ρ , x ↦ M) w ≡ M
map-≡ {_} {_} {w} {x} w≡ with w ≟ x
...                         | yes _    =  refl
...                         | no  w≢   =  ⊥-elim (w≢ w≡)

map-≢ : ∀ {ρ M w x} → w ≢ x → (ρ , x ↦ M) w ≡ ρ w
map-≢ {_} {_} {w} {x} w≢ with w ≟ x
...                         | yes w≡   =  ⊥-elim (w≢ w≡)
...                         | no  _    =  refl
\end{code}

\begin{code}
⊢subst : ∀ {Γ Δ ys ρ}
  → dom Δ ⊆ ys
  → (∀ {x A} → Γ ∋ x ⦂ A  →  Δ ⊢ ρ x ⦂ A)
    --------------------------------------------------------------
  → (∀ {M A} → Γ ⊢ M ⦂ A  →  Δ ⊢ subst ys ρ M ⦂ A)
⊢subst ⊆ys ⊢ρ (` ⊢x)
    =  ⊢ρ ⊢x
⊢subst {Γ} {Δ} {ys} {ρ} ⊆ys ⊢ρ (`λ_ {x = x} {A = A} {N = N} ⊢N)
    = `λ_ {x = y} {A = A} (⊢subst {Γ′} {Δ′} {ys′} {ρ′} ⊆ys′ ⊢ρ′ ⊢N)
  where
  y   =  fresh ys
  Γ′  =  Γ , x ⦂ A
  Δ′  =  Δ , y ⦂ A
  ys′ =  y ∷ ys
  ρ′  =  ρ , x ↦ ` y

  ⊆ys′ : dom Δ′ ⊆ ys′
  ⊆ys′ {w} here        =  here
  ⊆ys′ {w} (there w∈)  =  there (⊆ys w∈)

  ⊢σ : ∀ {w C} → Δ ∋ w ⦂ C → Δ′ ∋ w ⦂ C
  ⊢σ {w} ⊢w  =  S w≢ ⊢w
    where
    w≢ : w ≢ y
    w≢ = fresh-lemma (⊆ys (dom-lemma ⊢w))

  ⊢ρ′ : ∀ {w C} → Γ′ ∋ w ⦂ C → Δ′ ⊢ ρ′ w ⦂ C
  ⊢ρ′ {w} Z         rewrite map-≡ {ρ} {` y} {w} {x} refl  =  ` Z
  ⊢ρ′ {w} (S w≢ ⊢w) rewrite map-≢ {ρ} {` y} {w} {x} w≢    =  ⊢weaken {Δ} {Δ′} ⊢σ (⊢ρ ⊢w)

⊢subst Σ ⊢ρ (⊢L · ⊢M)
    =  ⊢subst Σ ⊢ρ ⊢L · ⊢subst Σ ⊢ρ ⊢M

{-
⊢subst : ∀ {Γ Δ xs ys ρ}
  → (∀ {x}   → x ∈ xs       →  free (ρ x) ⊆ ys)
  → (∀ {x A} → x ∈ xs       →  Γ ∋ x ⦂ A  →  Δ ⊢ ρ x ⦂ A)
    --------------------------------------------------------------
  → (∀ {M A} → free M ⊆ xs  →  Γ ⊢ M ⦂ A  →  Δ ⊢ subst ys ρ M ⦂ A)
⊢subst Σ ⊢ρ ⊆xs (` ⊢x)
    =  ⊢ρ (⊆xs here) ⊢x
⊢subst {Γ} {Δ} {xs} {ys} {ρ} Σ ⊢ρ ⊆xs (`λ_ {x = x} {A = A} {N = N} ⊢N)
    = `λ_ {x = y} {A = A} (⊢subst {Γ′} {Δ′} {xs′} {ys′} {ρ′} Σ′ ⊢ρ′ ⊆xs′ ⊢N)
  where
  y   =  fresh ys
  Γ′  =  Γ , x ⦂ A
  Δ′  =  Δ , y ⦂ A
  xs′ =  x ∷ xs
  ys′ =  y ∷ ys
  ρ′  =  ρ , x ↦ ` y

  Σ′ : ∀ {w} → w ∈ xs′ →  free (ρ′ w) ⊆ ys′
  Σ′ {w} w∈′ with w ≟ x
  ...            | yes refl    =  ⊆-++₁
  ...            | no  w≢      =  ⊆-++₂ ∘ Σ (there⁻¹ w∈′ w≢)

  ⊆xs′ :  free N ⊆ xs′
  ⊆xs′ =  \\-to-∷ ⊆xs

  ⊢σ : ∀ {w C} → w ∈ ys → Δ ∋ w ⦂ C → Δ′ ∋ w ⦂ C
  ⊢σ w∈ ⊢w  =  S (fresh-lemma w∈) ⊢w

  ⊢ρ′ : ∀ {w C} → w ∈ xs′ → Γ′ ∋ w ⦂ C → Δ′ ⊢ ρ′ w ⦂ C
  ⊢ρ′ {w} _ Z with w ≟ x
  ...         | yes _             =  ` Z
  ...         | no  w≢            =  ⊥-elim (w≢ refl)
  ⊢ρ′ {w} w∈′ (S w≢ ⊢w) with w ≟ x
  ...         | yes refl          =  ⊥-elim (w≢ refl)
  ...         | no  _             =  ⊢rename {Δ} {Δ′} {ys} ⊢σ (Σ w∈) (⊢ρ w∈ ⊢w)
              where
              w∈  =  there⁻¹ w∈′ w≢

⊢subst Σ ⊢ρ ⊆xs (⊢L · ⊢M)
    =  ⊢subst Σ ⊢ρ L⊆ ⊢L · ⊢subst Σ ⊢ρ M⊆ ⊢M
  where
  L⊆ = trans-⊆ ⊆-++₁ ⊆xs
  M⊆ = trans-⊆ ⊆-++₂ ⊆xs
-}
\end{code}

### Substitution preserves types, specific case

\begin{code}
infixl 5 _//_
_//_ : Env → List Id → Env
Γ // []                             =  Γ
ε // (y ∷ ys)                       =  ε
(Γ , x ⦂ A) // (y ∷ ys) with x ≟ y
...                        | yes _  =  Γ // ys , x ⦂ A
...                        | no  _  =  Γ // ys

//-lemma : ∀ {Γ xs} → dom (Γ // xs) ≡ xs
//-lemma = {!!}

⊢stronger : ∀ {Γ ys M A}
  → free M ⊆ ys
  → Γ ⊢ M ⦂ A
    -------------------
  → Γ // ys ⊢ M ⦂ A
⊢stronger = {!!}

⊢weaker : ∀ {Γ ys M A}
  → free M ⊆ ys
  → Γ // ys ⊢ M ⦂ A
    ---------------
  → Γ ⊢ M ⦂ A
⊢weaker = {!!}

⊢substitution₀ : ∀ {Δ x A N B M}
  → dom Δ ⊆ free M ++ (free N \\ x)
  → Δ , x ⦂ A ⊢ N ⦂ B
  → Δ ⊢ M ⦂ A
    ---------------------
  → Δ ⊢ N [ x := M ] ⦂ B
⊢substitution₀ = {!!}

{-
⊢substitution : ∀ {Γ x A N B M}
  → Γ , x ⦂ A ⊢ N ⦂ B
  → Γ ⊢ M ⦂ A
    --------------------
  → Γ ⊢ N [ x := M ] ⦂ B
⊢substitution {Γ} {x} {A} {N} {B} {M} ⊢N ⊢M =
  ⊢weaker {Γ} {ys} ⊆N[x:=M]
    (⊢substitution₀
      (refl-⊆ (//-lemma {Γ} {ys}))
      (⊢stronger {Γ , x ⦂ A} {x ∷ ys} ⊆N ⊢N)
      (⊢stronger {Γ} {ys} ⊆M ⊢M))
    where
    ys = free M ++ (free N \\ x)
    ⊆N : free N ⊆ x ∷ ys
    ⊆N = ?
    ⊆M : free M ⊆ ys
    ⊆M = ?
    ⊆N[x:=M] : free (N [ x := M ]) ⊆ ys
    ⊆N[x:=M] = ?
-}

{-
⊢substitution : ∀ {Γ x A N B M} →
  Γ , x ⦂ A ⊢ N ⦂ B →
  Γ ⊢ M ⦂ A →
  --------------------
  Γ ⊢ N [ x := M ] ⦂ B
⊢substitution {Γ} {x} {A} {N} {B} {M} ⊢N ⊢M =
  subst {Γ′ , x ⦂ A} {Γ′} {ys} {ρ} Σ ⊢ρ ⊢N′
  where
  ys   =  free M ++ (free N \\ x)
  Δ    =  Γ // ys
  ⊢N′  =  rename {Γ , x ⦂ A} {Δ , x ⦂ A} ? ⊢N
  ⊢M′  =  rename {Γ} {Δ} ? ⊢M

  -- rename is no longer sufficiently powerful
  -- it can do weakening but not strengthening

  -- not clear where and how def'n of ys gets used

  ⊢subst {Γ′} {Γ} {xs} {ys} {ρ} Σ ⊢ρ {N} {B} ⊆xs ⊢N
  where
  Γ′     =  Γ , x ⦂ A
  xs     =  free N
  ρ      =  ∅ , x ↦ M

  Σ : ∀ {w} → w ∈ xs → free (ρ w) ⊆ ys
  Σ {w} w∈ y∈ with w ≟ x
  ...            | yes _                   =  ⊆-++₁ y∈
  ...            | no w≢ rewrite ∈-[_] y∈  =  ⊆-++₂ (∈-≢-to-\\ w∈ w≢)

  ⊢ρ : ∀ {w B} → w ∈ xs → Γ′ ∋ w ⦂ B → Γ ⊢ ρ w ⦂ B
  ⊢ρ {w} w∈ Z         with w ≟ x
  ...                    | yes _     =  ⊢M
  ...                    | no  w≢    =  ⊥-elim (w≢ refl)
  ⊢ρ {w} w∈ (S w≢ ⊢w) with w ≟ x
  ...                    | yes refl  =  ⊥-elim (w≢ refl)
  ...                    | no  _     =  ` ⊢w

  ⊆xs : free N ⊆ xs
  ⊆xs x∈ = x∈
-}

{-
⊢substitution : ∀ {Γ x A N B M} →
  Γ , x ⦂ A ⊢ N ⦂ B →
  Γ ⊢ M ⦂ A →
  --------------------
  Γ ⊢ N [ x := M ] ⦂ B
⊢substitution {Γ} {x} {A} {N} {B} {M} ⊢N ⊢M =
  subst {Γ′ , x ⦂ A} {Γ′} {ys} {ρ} Σ ⊢ρ ⊢N′
  where
  ys   =  free M ++ (free N \\ x)
  Γ′   =  Γ // ys
  ⊢N′  =  rename {Γ , x ⦂ A} {Γ′ , x ⦂ A} ? ⊢N
  ⊢M′  =  rename {Γ} {Γ′} ? ⊢M

  -- rename is no longer sufficiently powerful
  -- it can do weakening but not strengthening

  -- not clear where and how def'n of ys gets used

  ⊢subst {Γ′} {Γ} {xs} {ys} {ρ} Σ ⊢ρ {N} {B} ⊆xs ⊢N
  where
  Γ′     =  Γ , x ⦂ A
  xs     =  free N
  ρ      =  ∅ , x ↦ M

  Σ : ∀ {w} → w ∈ xs → free (ρ w) ⊆ ys
  Σ {w} w∈ y∈ with w ≟ x
  ...            | yes _                   =  ⊆-++₁ y∈
  ...            | no w≢ rewrite ∈-[_] y∈  =  ⊆-++₂ (∈-≢-to-\\ w∈ w≢)

  ⊢ρ : ∀ {w B} → w ∈ xs → Γ′ ∋ w ⦂ B → Γ ⊢ ρ w ⦂ B
  ⊢ρ {w} w∈ Z         with w ≟ x
  ...                    | yes _     =  ⊢M
  ...                    | no  w≢    =  ⊥-elim (w≢ refl)
  ⊢ρ {w} w∈ (S w≢ ⊢w) with w ≟ x
  ...                    | yes refl  =  ⊥-elim (w≢ refl)
  ...                    | no  _     =  ` ⊢w

  ⊆xs : free N ⊆ xs
  ⊆xs x∈ = x∈
-}

{-
⊢substitution : ∀ {Γ x A N B M} →
  Γ , x ⦂ A ⊢ N ⦂ B →
  Γ ⊢ M ⦂ A →
  --------------------
  Γ ⊢ N [ x := M ] ⦂ B
⊢substitution {Γ} {x} {A} {N} {B} {M} ⊢N ⊢M =
  ⊢subst {Γ′} {Γ} {xs} {ys} {ρ} Σ ⊢ρ {N} {B} ⊆xs ⊢N
  where
  Γ′     =  Γ , x ⦂ A
  xs     =  free N
  ys     =  free M ++ (free N \\ x)
  ρ      =  ∅ , x ↦ M

  Σ : ∀ {w} → w ∈ xs → free (ρ w) ⊆ ys
  Σ {w} w∈ y∈ with w ≟ x
  ...            | yes _                   =  ⊆-++₁ y∈
  ...            | no w≢ rewrite ∈-[_] y∈  =  ⊆-++₂ (∈-≢-to-\\ w∈ w≢)

  ⊢ρ : ∀ {w B} → w ∈ xs → Γ′ ∋ w ⦂ B → Γ ⊢ ρ w ⦂ B
  ⊢ρ {w} w∈ Z         with w ≟ x
  ...                    | yes _     =  ⊢M
  ...                    | no  w≢    =  ⊥-elim (w≢ refl)
  ⊢ρ {w} w∈ (S w≢ ⊢w) with w ≟ x
  ...                    | yes refl  =  ⊥-elim (w≢ refl)
  ...                    | no  _     =  ` ⊢w

  ⊆xs : free N ⊆ xs
  ⊆xs x∈ = x∈
-}
\end{code}

### Preservation

\begin{code}
{-
preservation : ∀ {Γ M N A}
  →  Γ ⊢ M ⦂ A
  →  M ⟶ N
     ---------
  →  Γ ⊢ N ⦂ A
preservation (` ⊢x) ()
preservation (`λ ⊢N) ()
preservation (⊢L · ⊢M) (ξ-⟹₁ L⟶L′)        =  preservation ⊢L L⟶L′ · ⊢M
preservation (⊢V · ⊢M) (ξ-⟹₂ valV M⟶M′)   =  ⊢V · preservation ⊢M M⟶M′
preservation ((`λ ⊢N) · ⊢W) (β-⟹ valW)      =  ⊢substitution ⊢N ⊢W
-}
\end{code}



